Protocols/ABC/Liveness_tla.v
@@ -6,15 +6,15 @@ From ABCProtocol.Protocols.ABC Require Export Liveness.
 
 From ABCProtocol.Properties Require Export Liveness_tla.
 
-Module ACLiveness2 (A : NetAddr) (Sn : Signable) (V : SignableValue Sn) (VBFT : ValueBFT A Sn V) 
+Module ACLiveness2 (A : NetAddr) (Sn : Signable) (V : SignableValue Sn) (* (VBFT : ValueBFT A Sn V) *)
   (BTh : ByzThreshold A) (BSett : ByzSetting A)
   (P : PKI A Sn) (TSS0 : ThresholdSignatureSchemePrim A Sn with Definition thres := BTh.t0) (* ! *)
   (TSS : ThresholdSignatureScheme A Sn with Module TSSPrim := TSS0).
 
-Import A V VBFT BTh BSett P TSS.
+Import A V (* VBFT *) BTh BSett P TSS.
 Import ssrbool. (* anyway *)
 
-Module Export ACLive := ACLiveness A Sn V VBFT BTh BSett P TSS0 TSS.
+Module Export ACLive := ACLiveness A Sn V (* VBFT *) BTh BSett P TSS0 TSS.
 Include LivenessTLA A M BTh BSett P0 PSOp ACP Ns ACAdv ACN.
 
 Section A.
@@ -43,7 +43,14 @@ Proof.
   let tac n := rewrite <- exist_state_pred; apply leads_to_exist_intro; intros n in tac n1; tac n2.
   tla_apply (leads_to_trans _ (⌜ round_2_start n1 n2 ⌝)). tla_split.
   - delivering round_1_pkts which ends at round_1_end_suffcond is sufficient because round_2_start_suffcond.
-  - delivering round_2_pkts which ends at round_2_end_suffcond is sufficient because accountability_suffcond.
+  - (* TODO automation broken ... but not quite want to fix now *) 
+    apply leads_to_by_eventual_delivery.
+    intros. pose proof round_2_pkts as Htmp. saturate_assumptions!.
+    destruct Htmp as (pkts & Htmp). hnf in Htmp. exists pkts.
+    destruct (w @ n1).(submitted_value) eqn:E1, (w @ n2).(submitted_value) eqn:E2; try contradiction. 
+    hnf in Htmp. destruct_and? Htmp.
+    split_and?; auto. intros. simplify_eq. eapply accountability_suffcond; eauto; eapply round_2_end_suffcond; hnf; eauto.
+    rewrite E1 E2. now hnf.
 Qed.
 
 End A.
